messageInvariantPrototypes/ringLeaderElection/centralized/applicationProof.dfy
@@ -48,10 +48,10 @@ ghost predicate ChordDominates(c: Constants, v: Variables)
       && c.ValidIdx(src)
       && c.ValidIdx(dst)
       && c.ValidIdx(mid)
-      && v.hosts[dst].highestHeard == c.hostConstants[src].hostId
+      && v.hosts[dst].highestHeard == c.hosts[src].hostId
       && Between(src, mid, dst)
     :: 
-      c.hostConstants[mid].hostId < c.hostConstants[src].hostId
+      c.hosts[mid].hostId < c.hosts[src].hostId
 }
 
 
